Engine: fix boolean semantics with the new strict suffix semantics

Engine/BooleanSemantics.v
@@ -4,6 +4,7 @@ Import ListNotations.
 From Linden Require Import Regex Chars Groups.
 From Linden Require Import Tree Semantics PikeSubset.
 From Warblre Require Import Base.
+From Linden Require Import StrictSuffix.
 
 
 (* An alternate definition of the semantics, using a boolean to know if one can exit a loop *)
@@ -115,46 +116,8 @@ Inductive LoopBool : Type :=
 
 
 (** * First Step: encoding the invariant  *)
-Definition suffix (str1 str2:string) : Prop :=
-  exists prefix, str2 = prefix ++ str1.
 
-Definition strict_suffix (str1 str2:string) : Prop :=
-  suffix str1 str2 /\ str1 <> str2.
-
-Lemma cons_neq:
-  forall A str pref (c:A),
-    str = pref ++ c::str -> False.
-Proof.
-  intros A str pref c H.
-  assert (List.length str = List.length pref + 1 + List.length str).
-  { rewrite H at 1. rewrite app_length. simpl. lia. }
-  lia.
-Qed.
-
-Lemma strict_cons:
-  forall s c,
-    strict_suffix s (c::s).
-Proof.
-  intros s c. unfold strict_suffix, suffix. split.
-  - exists [c]. simpl. auto.
-  - unfold not.
-    replace (c::s) with ([] ++ c::s) by auto.
-    apply cons_neq.
-Qed.    
-
-Lemma strict_app:
-  forall str1 str2 c,
-    strict_suffix (c::str1) str2 ->
-    strict_suffix str1 str2.
-Proof.
-  unfold strict_suffix, suffix. intros str2 str0 c [[prefix APP] NEQ].
-  split.
-  - exists (prefix ++ [c]). rewrite <- app_assoc. simpl. auto.
-  - unfold not. intros H. subst. eapply cons_neq; eauto.
-Qed.
-  
-
-Inductive bool_encoding: LoopBool -> input -> actions -> Prop :=
+ Inductive bool_encoding: LoopBool -> input -> actions -> Prop :=
 (* an empty continuation can be encoded with any boolean *)
 | nil_encode:
   forall str b,
@@ -170,7 +133,7 @@ Inductive bool_encoding: LoopBool -> input -> actions -> Prop :=
 | cons_true:
   forall stk str head 
     (ENCODE: bool_encoding CanExit str stk)
-    (STRICT: strict_suffix (current_str str forward) (current_str head forward)),
+    (STRICT: strict_suffix str head forward),
     bool_encoding CanExit str (Acheck head::stk)
 | cons_false:
   (* when we push the current string to the stack *)
@@ -192,10 +155,12 @@ Proof.
   - constructor.
   - constructor; auto.
   - constructor; auto.
-  - constructor; auto. rewrite Heqprevstr in STRICT. eapply strict_app; eauto.
+  - constructor; auto. rewrite Heqprevstr in STRICT.
+    eapply ss_next; eauto. simpl. auto.
   - constructor.
     + apply IHbool_encoding; auto.
-    + subst. simpl. apply strict_cons.
+    + subst. simpl.
+      eapply ss_advance; eauto.
 Qed.
 
 (* if the string is different than the check, we know the boolean is true *)
@@ -219,8 +184,7 @@ Proof.
   intros b str cont H.
   remember (Acheck str::cont) as prevcont.
   induction H; intros; auto; inversion Heqprevcont.
-  subst. destruct STRICT as [_ NEQ].
-  exfalso. apply NEQ. auto.
+  subst. apply ss_neq in STRICT. contradiction. 
 Qed.
 
 Lemma encode_next:
@@ -252,9 +216,16 @@ Lemma encoding_suffix:
   forall b inp act chk,
     bool_encoding b inp act ->
     In (Acheck chk) act ->
-    inp = chk \/ StrictSuffix.strict_suffix inp chk forward.
+    inp = chk \/ strict_suffix inp chk forward.
 Proof.
-Admitted.
+  intros. induction H.
+  - inversion H0.
+  - simpl in H0. destruct H0 as [H0|IN]; try inversion H0; auto.
+  - simpl in H0. destruct H0 as [H0|IN]; try inversion H0; auto.
+  - simpl in H0. destruct H0 as [H0|IN]; try inversion H0; auto.
+    right. subst. auto.
+  - simpl in H0. destruct H0 as [H0|IN]; try inversion H0; auto.
+Qed.
 
 
 (** * Second Step: encoding equality  *)
@@ -274,10 +245,10 @@ Proof.
     try solve[constructor; auto]; try solve [inversion H1; inversion H0].
   - assert (b = CanExit).
     { eapply encoding_different; eauto.
-      eapply StrictSuffix.ss_neq; eauto. }
+      eapply ss_neq; eauto. }
     subst. constructor. eapply IHTREE; eauto.
     inversion ENCODE; subst; auto.
-  - assert (inp = strcheck \/ StrictSuffix.strict_suffix inp strcheck forward).
+  - assert (inp = strcheck \/ strict_suffix inp strcheck forward).
     { eapply encoding_suffix; eauto. simpl. auto. }
     destruct H; try contradiction. subst.
     assert (b = CannotExit).
@@ -415,4 +386,3 @@ Qed.
     - apply bool_to_istree; auto.
     - apply boolean_correct; auto.
   Qed.
-
